nonlinear: represent centered Taylor analytic programs

candle/cv_compute_analytic_expr_taylor_model_representation.ml
@@ -927,4 +927,265 @@ let candle_cv_q_dim_taylor_model_poly_program_correct = prove
               candle_cv_q_dim_taylor_model_poly_run_correct;
               candle_cv_q_dim_taylor_model_result_head_correct]);;
 
+(* A small ordinary decoder mirrors the two cval instruction shapes.  Tags  *)
+(* 0 and 1 are paired payload instructions; tags 2--8 are nullary nodes.     *)
+
+let candle_q_analytic_instruction_tag_def = define
+ `(candle_q_analytic_instruction_tag
+      (Candle_analytic_push_poly program) = 0) /\
+  (candle_q_analytic_instruction_tag Candle_analytic_program_neg = 2) /\
+  (candle_q_analytic_instruction_tag Candle_analytic_program_add = 3) /\
+  (candle_q_analytic_instruction_tag Candle_analytic_program_mul = 4) /\
+  (candle_q_analytic_instruction_tag Candle_analytic_program_square = 5) /\
+  (candle_q_analytic_instruction_tag Candle_analytic_program_inv = 6) /\
+  (candle_q_analytic_instruction_tag
+      (Candle_analytic_program_sqrt s) = 1) /\
+  (candle_q_analytic_instruction_tag Candle_analytic_program_atn = 7) /\
+  (candle_q_analytic_instruction_tag Candle_analytic_program_pi_half = 8)`;;
+
+let candle_q_analytic_instruction_poly_def = define
+ `(candle_q_analytic_instruction_poly
+      (Candle_analytic_push_poly program) = program) /\
+  (candle_q_analytic_instruction_poly Candle_analytic_program_neg = []) /\
+  (candle_q_analytic_instruction_poly Candle_analytic_program_add = []) /\
+  (candle_q_analytic_instruction_poly Candle_analytic_program_mul = []) /\
+  (candle_q_analytic_instruction_poly Candle_analytic_program_square = []) /\
+  (candle_q_analytic_instruction_poly Candle_analytic_program_inv = []) /\
+  (candle_q_analytic_instruction_poly
+      (Candle_analytic_program_sqrt s) = []) /\
+  (candle_q_analytic_instruction_poly Candle_analytic_program_atn = []) /\
+  (candle_q_analytic_instruction_poly
+      Candle_analytic_program_pi_half = [])`;;
+
+let candle_q_analytic_instruction_sqrt_def = define
+ `(candle_q_analytic_instruction_sqrt
+      (Candle_analytic_push_poly program) = candle_q_zero_interval) /\
+  (candle_q_analytic_instruction_sqrt
+      Candle_analytic_program_neg = candle_q_zero_interval) /\
+  (candle_q_analytic_instruction_sqrt
+      Candle_analytic_program_add = candle_q_zero_interval) /\
+  (candle_q_analytic_instruction_sqrt
+      Candle_analytic_program_mul = candle_q_zero_interval) /\
+  (candle_q_analytic_instruction_sqrt
+      Candle_analytic_program_square = candle_q_zero_interval) /\
+  (candle_q_analytic_instruction_sqrt
+      Candle_analytic_program_inv = candle_q_zero_interval) /\
+  (candle_q_analytic_instruction_sqrt
+      (Candle_analytic_program_sqrt s) = s) /\
+  (candle_q_analytic_instruction_sqrt
+      Candle_analytic_program_atn = candle_q_zero_interval) /\
+  (candle_q_analytic_instruction_sqrt
+      Candle_analytic_program_pi_half = candle_q_zero_interval)`;;
+
+let candle_q_dim_taylor_model_program_step_def = new_definition
+ `candle_q_dim_taylor_model_program_step
+      center_boxes boxes radii center_instruction box_instruction stack =
+    if candle_q_analytic_instruction_tag center_instruction = 0 then
+      (if candle_q_analytic_instruction_tag box_instruction = 0 then
+         CONS
+           (candle_q_dim_taylor_model_poly_program
+             center_boxes boxes radii
+             (candle_q_analytic_instruction_poly center_instruction)) stack
+       else CONS
+         (candle_q_dim_taylor_model_result_default center_boxes boxes) stack)
+    else if candle_q_analytic_instruction_tag center_instruction = 1 then
+      (if candle_q_analytic_instruction_tag box_instruction = 1 then
+         CONS
+           (candle_q_dim_taylor_model_result_sqrt radii
+             (candle_q_analytic_instruction_sqrt center_instruction)
+             (candle_q_analytic_instruction_sqrt box_instruction)
+             (candle_q_dim_taylor_model_result_head
+               center_boxes boxes stack))
+           (candle_q_dim_taylor_model_result_tail stack)
+       else CONS
+         (candle_q_dim_taylor_model_result_default center_boxes boxes) stack)
+    else if candle_q_analytic_instruction_tag box_instruction < 2 then
+      CONS (candle_q_dim_taylor_model_result_default center_boxes boxes) stack
+    else if candle_q_analytic_instruction_tag center_instruction =
+            candle_q_analytic_instruction_tag box_instruction then
+      if candle_q_analytic_instruction_tag center_instruction = 2 then
+        CONS
+          (candle_q_dim_taylor_model_result_neg radii
+            (candle_q_dim_taylor_model_result_head
+              center_boxes boxes stack))
+          (candle_q_dim_taylor_model_result_tail stack)
+      else if candle_q_analytic_instruction_tag center_instruction = 3 then
+        CONS
+          (candle_q_dim_taylor_model_result_add radii
+            (candle_q_dim_taylor_model_result_head center_boxes boxes
+              (candle_q_dim_taylor_model_result_tail stack))
+            (candle_q_dim_taylor_model_result_head
+              center_boxes boxes stack))
+          (candle_q_dim_taylor_model_result_tail
+            (candle_q_dim_taylor_model_result_tail stack))
+      else if candle_q_analytic_instruction_tag center_instruction = 4 then
+        CONS
+          (candle_q_dim_taylor_model_result_mul radii
+            (candle_q_dim_taylor_model_result_head center_boxes boxes
+              (candle_q_dim_taylor_model_result_tail stack))
+            (candle_q_dim_taylor_model_result_head
+              center_boxes boxes stack))
+          (candle_q_dim_taylor_model_result_tail
+            (candle_q_dim_taylor_model_result_tail stack))
+      else if candle_q_analytic_instruction_tag center_instruction = 5 then
+        CONS
+          (candle_q_dim_taylor_model_result_square radii
+            (candle_q_dim_taylor_model_result_head
+              center_boxes boxes stack))
+          (candle_q_dim_taylor_model_result_tail stack)
+      else if candle_q_analytic_instruction_tag center_instruction = 6 then
+        CONS
+          (candle_q_dim_taylor_model_result_inv radii
+            (candle_q_dim_taylor_model_result_head
+              center_boxes boxes stack))
+          (candle_q_dim_taylor_model_result_tail stack)
+      else if candle_q_analytic_instruction_tag center_instruction = 7 then
+        CONS
+          (candle_q_dim_taylor_model_result_atn radii
+            (candle_q_dim_taylor_model_result_head
+              center_boxes boxes stack))
+          (candle_q_dim_taylor_model_result_tail stack)
+      else if candle_q_analytic_instruction_tag center_instruction = 8 then
+        CONS
+          (candle_q_dim_taylor_model_result_pi_half
+            radii center_boxes boxes) stack
+      else CONS
+        (candle_q_dim_taylor_model_result_default center_boxes boxes) stack
+    else CONS
+      (candle_q_dim_taylor_model_result_default center_boxes boxes) stack`;;
+
+let candle_cv_q_dim_taylor_model_program_step_correct = prove
+ (`!center_instruction box_instruction center_boxes boxes radii stack.
+     candle_cv_q_dim_taylor_model_program_step
+       (candle_cv_q_interval_list center_boxes)
+       (candle_cv_q_interval_list boxes)
+       (candle_cv_q_list radii)
+       (candle_cv_analytic_instruction center_instruction)
+       (candle_cv_analytic_instruction box_instruction)
+       (candle_cv_q_dim_taylor_model_result_list_encode stack) =
+     candle_cv_q_dim_taylor_model_result_list_encode
+       (candle_q_dim_taylor_model_program_step center_boxes boxes radii
+         center_instruction box_instruction stack)`,
+  REPEAT GEN_TAC THEN
+  STRUCT_CASES_TAC
+    (SPEC `center_instruction:candle_analytic_instruction`
+      (cases "candle_analytic_instruction")) THEN
+  STRUCT_CASES_TAC
+    (SPEC `box_instruction:candle_analytic_instruction`
+      (cases "candle_analytic_instruction")) THEN
+  REWRITE_TAC[candle_cv_q_dim_taylor_model_program_step_def;
+              candle_q_dim_taylor_model_program_step_def;
+              candle_cv_analytic_instruction_def;
+              candle_q_analytic_instruction_tag_def;
+              candle_q_analytic_instruction_poly_def;
+              candle_q_analytic_instruction_sqrt_def;
+              candle_cv_q_dim_taylor_model_result_list_encode_def;
+              cexp_fst_def; cexp_snd_def; cexp_eq_def; cexp_if_def;
+              cexp_ispair_def; distinctness "cval"; injectivity "cval";
+              NOT_SUC; candle_one_ne_zero; candle_four_ne_two;
+              candle_four_ne_three; candle_three_ne_two;
+              candle_five_ne_two; candle_five_ne_three;
+              candle_five_ne_four; candle_six_ne_two;
+              candle_six_ne_three; candle_six_ne_four;
+              candle_six_ne_five;
+              candle_seven_ne_two; candle_seven_ne_three;
+              candle_seven_ne_four; candle_seven_ne_five;
+              candle_seven_ne_six;
+              candle_eight_ne_two; candle_eight_ne_three;
+              candle_eight_ne_four; candle_eight_ne_five;
+              candle_eight_ne_six; candle_eight_ne_seven;
+              candle_cv_q_dim_taylor_model_poly_program_correct;
+              candle_cv_q_dim_taylor_model_result_default_correct;
+              candle_cv_q_dim_taylor_model_result_head_correct;
+              candle_cv_q_dim_taylor_model_result_tail_correct;
+              candle_cv_q_dim_taylor_model_result_neg_correct;
+              candle_cv_q_dim_taylor_model_result_add_correct;
+              candle_cv_q_dim_taylor_model_result_mul_correct;
+              candle_cv_q_dim_taylor_model_result_square_correct;
+              candle_cv_q_dim_taylor_model_result_inv_correct;
+              candle_cv_q_dim_taylor_model_result_sqrt_correct;
+              candle_cv_q_dim_taylor_model_result_atn_correct;
+              candle_cv_q_dim_taylor_model_result_pi_half_correct] THEN
+  CONV_TAC NUM_REDUCE_CONV THEN
+  REWRITE_TAC[candle_cv_q_dim_taylor_model_result_list_encode_def]);;
+
+let candle_q_dim_taylor_model_program_run_def = define
+ `(candle_q_dim_taylor_model_program_run
+      center_boxes boxes radii [] box_program stack = stack) /\
+  (candle_q_dim_taylor_model_program_run
+      center_boxes boxes radii (CONS ch ct) [] stack = stack) /\
+  (candle_q_dim_taylor_model_program_run
+      center_boxes boxes radii (CONS ch ct) (CONS bh bt) stack =
+     candle_q_dim_taylor_model_program_run
+       center_boxes boxes radii ct bt
+       (candle_q_dim_taylor_model_program_step
+         center_boxes boxes radii ch bh stack))`;;
+
+let candle_cv_q_dim_taylor_model_program_run_correct = prove
+ (`!center_program box_program center_boxes boxes radii stack.
+     candle_cv_q_dim_taylor_model_program_run
+       (candle_cv_q_interval_list center_boxes)
+       (candle_cv_q_interval_list boxes)
+       (candle_cv_q_list radii)
+       (candle_cv_analytic_instruction_list center_program)
+       (candle_cv_analytic_instruction_list box_program)
+       (candle_cv_q_dim_taylor_model_result_list_encode stack) =
+     candle_cv_q_dim_taylor_model_result_list_encode
+       (candle_q_dim_taylor_model_program_run
+         center_boxes boxes radii center_program box_program stack)`,
+  LIST_INDUCT_TAC THENL
+   [REPEAT GEN_TAC THEN
+    REWRITE_TAC[candle_cv_analytic_instruction_list_def;
+                candle_cv_q_dim_taylor_model_program_run_def;
+                candle_q_dim_taylor_model_program_run_def];
+    LIST_INDUCT_TAC THEN REPEAT GEN_TAC THEN
+    ASM_REWRITE_TAC[candle_cv_analytic_instruction_list_def;
+                    candle_cv_q_dim_taylor_model_program_run_def;
+                    candle_q_dim_taylor_model_program_run_def;
+                    candle_cv_q_dim_taylor_model_program_step_correct]]);;
+
+let candle_q_fixed_list_round_upper_def = define
+ `(candle_q_fixed_list_round_upper [] = []) /\
+  (candle_q_fixed_list_round_upper (CONS h t) =
+     CONS (candle_q_fixed_round_upper h)
+       (candle_q_fixed_list_round_upper t))`;;
+
+let candle_cv_q_fixed_list_round_upper_correct = prove
+ (`!items.
+     candle_cv_q_fixed_list_round_upper (candle_cv_q_list items) =
+     candle_cv_q_list (candle_q_fixed_list_round_upper items)`,
+  LIST_INDUCT_TAC THEN
+  ASM_REWRITE_TAC[candle_cv_q_fixed_list_round_upper_def;
+                  candle_q_fixed_list_round_upper_def;
+                  candle_cv_q_list_def;
+                  candle_cv_q_fixed_round_upper_correct]);;
+
+let candle_q_dim_taylor_model_program_def = new_definition
+ `candle_q_dim_taylor_model_program center_program box_program boxes =
+    candle_q_dim_taylor_model_result_head
+      (candle_q_center_environment_list boxes) boxes
+      (candle_q_dim_taylor_model_program_run
+        (candle_q_center_environment_list boxes) boxes
+        (candle_q_fixed_list_round_upper (candle_q_radius_list boxes))
+        center_program box_program [])`;;
+
+let candle_cv_q_dim_taylor_model_program_correct = prove
+ (`!center_program box_program boxes.
+     candle_cv_q_dim_taylor_model_program
+       (candle_cv_analytic_instruction_list center_program)
+       (candle_cv_analytic_instruction_list box_program)
+       (candle_cv_q_interval_list boxes) =
+     candle_cv_q_dim_taylor_model_result_encode
+       (candle_q_dim_taylor_model_program
+         center_program box_program boxes)`,
+  REPEAT GEN_TAC THEN
+  REWRITE_TAC[candle_cv_q_dim_taylor_model_program_def;
+              candle_q_dim_taylor_model_program_def;
+              candle_cv_q_center_environment_list_correct;
+              candle_cv_q_radius_list_correct;
+              candle_cv_q_fixed_list_round_upper_correct;
+              GSYM candle_cv_q_dim_taylor_model_result_list_encode_def;
+              candle_cv_q_dim_taylor_model_program_run_correct;
+              candle_cv_q_dim_taylor_model_result_head_correct]);;
+
 end;;
